theories/case_studies/multiuser_kvs/kvs_initialise.v
@@ -1,0 +1,278 @@
+From iris.proofmode Require Import proofmode.
+From griotte Require Import proofmode map_simpl.
+From griotte Require Import logrel rules.
+From griotte Require Import region_invariants_revocation wp_rules_interp interp_weakening.
+From griotte Require Import switcher_preamble switcher_spec_return.
+From griotte Require Import switcher fetch_spec kvs kvs_preamble.
+
+
+
+Section KVS_spec_initialise.
+  Context
+    {Σ:gFunctors}
+    {ceriseg:ceriseG Σ} {sealsg: sealStoreG Σ}
+    {Cname : CmptNameG}
+    {stsg : STSG Addr region_type OType Word Σ} {relg : relGS Σ}
+    {kvsg:kvsG Σ}
+    {cstackg : CSTACKG Σ}
+    `{MP: MachineParameters}
+    {swlayout : switcherLayout}
+    {KVS_layout : kvsLayout} {KVS_layout_WF : kvsLayoutWf} {KVS_users: kvs_users} {KVS_namespaces : kvs_namespaces}
+  .
+
+  Lemma KVS_initialise_spec_pre
+    (pc_b pc_e pc_a : Addr)
+    (cgp_b cgp_e : Addr)
+    (wret : Word)
+    (next_free_uk : Z)
+    :
+
+
+    SubBounds pc_b pc_e pc_a (pc_a ^+ length kvs_initialise_instrs)%a ->
+
+    (cgp_b + length_kvs_data)%a = Some cgp_e ->
+
+    (
+      (* initial register file *)
+      PC ↦ᵣ WCap RX Global pc_b pc_e pc_a ∗
+      cgp ↦ᵣ WCap RW Global cgp_b cgp_e cgp_b ∗
+      cra ↦ᵣ wret ∗
+      ca0 ↦ᵣ - ∗
+      ca1 ↦ᵣ - ∗
+      ct0 ↦ᵣ - ∗ (* scratch *)
+      ct1 ↦ᵣ - ∗ (* scratch *)
+      ctp ↦ᵣ - ∗ (* scratch *)
+      cnull ↦ᵣ - ∗
+
+      (* initial memory layout *)
+      codefrag pc_a kvs_initialise_instrs ∗
+      (pc_b ^+ UNSEALING_USER_KEY_OFFSET)%a ↦ₐ kvs_service_unsealing_key ∗
+      (cgp_b ^+ OFFSET_NEXT_FREE_SEALED_USER_KEY)%a ↦ₐ (kvs_user_seal_key_scap_init next_free_uk) ∗
+
+      ▷ ([∗ list] uk ∈ (seqZ next_free_uk (MemNum - next_free_uk)%Z), ◯(ALLOC)[uk] ∅) ∗
+
+      ▷ (PC ↦ᵣ updatePcPerm wret ∗
+         cgp ↦ᵣ - ∗
+         cra ↦ᵣ - ∗
+         ca0 ↦ᵣ WInt (if ( next_free_uk <? MemNum)%Z then ASM_SOME else ASM_NONE) ∗
+         (
+           if ( next_free_uk <? MemNum)%Z
+           then ca1 ↦ᵣ (kvs_user_seal_key Global next_free_uk)
+           else ca1 ↦ᵣ -
+         ) ∗ (* result of the initialise *)
+         ct0 ↦ᵣ - ∗ (* scratch *)
+         ct1 ↦ᵣ - ∗ (* scratch *)
+         ctp ↦ᵣ - ∗ (* scratch *)
+         cnull ↦ᵣ - ∗
+
+         codefrag pc_a kvs_initialise_instrs ∗
+         (pc_b ^+ UNSEALING_USER_KEY_OFFSET)%a ↦ₐ kvs_service_unsealing_key ∗
+         (cgp_b ^+ OFFSET_NEXT_FREE_SEALED_USER_KEY)%a ↦ₐ
+           (kvs_user_seal_key_scap_init
+              (if ( next_free_uk <? MemNum)%Z
+               then (next_free_uk + 1)%Z
+               else next_free_uk)
+           ) ∗
+
+         (
+           if ( next_free_uk <? MemNum)%Z
+           then ( ([∗ list] uk ∈ (seqZ (next_free_uk + 1) (MemNum - (next_free_uk + 1))), ◯(ALLOC)[uk] ∅) ∗ ◯(ALLOC)[next_free_uk] ∅)
+           else ([∗ list] uk ∈ (seqZ next_free_uk (MemNum - next_free_uk)%Z), ◯(ALLOC)[uk] ∅)
+         )
+
+         -∗ WP Seq (Instr Executable) {{ v, ⌜v = HaltedV⌝ → na_own cerise_nais ⊤ }}
+        )
+      ⊢ WP Seq (Instr Executable) {{ v, ⌜v = HaltedV⌝ → na_own cerise_nais ⊤ }})%I.
+  Proof.
+    iIntros (HsubBounds Hcgp_contiguous)
+      "(HPC & Hcgp & Hcra & [%wca0 Hca0] & [%wca1 Hca1] & [%wct0 Hct0] & [%wct1 Hct1] & [%wctp Hctp] & [%wcnull Hcnull] & Hcode
+      & Ha_unsealing & Ha_next_free_uk & Hnext_free_alloc & Hpost)".
+    rewrite /length_kvs_data /= in Hcgp_contiguous.
+    codefrag_facts "Hcode"; rename H into Hpc_contiguous ; clear H0.
+
+    (* --------------------------------------------------- *)
+    (* ----------------- Start the proof ----------------- *)
+    (* --------------------------------------------------- *)
+    rewrite /kvs_initialise_instrs /assembled_kvs_initialise.
+    (* rewrite -/(fetch_instrs UNSEALING_USER_KEY_OFFSET ct0 ctp ct1). *)
+
+    focus_block_0 "Hcode" as "Hcode" "Hcont"; iHide "Hcont" as hcont.
+    iApply (fetch_spec with "[- $HPC $Hct0 $Hctp $Hct1 $Ha_unsealing $Hcode]"); eauto.
+    { rewrite /UNSEALING_USER_KEY_OFFSET; solve_addr. }
+    iNext ; iIntros "(HPC & Hct0 & Hctp & Hct1 & Hcode & Ha_unsealing)".
+    iEval (cbn) in "Hct0".
+    subst hcont; unfocus_block "Hcode" "Hcont" as "Hcode".
+
+    focus_block 1 "Hcode" as a_initialise Ha_initialise "Hcode" "Hcont". iHide "Hcont" as hcont.
+    (* lea cgp OFFSET_NEXT_FREE_SEALED_USER_KEY; *)
+    iInstr "Hcode".
+    { transitivity (Some (cgp_b ^+ OFFSET_NEXT_FREE_SEALED_USER_KEY)%a); auto; solve_addr. }
+    (* load ct1 cgp; *)
+    iInstr "Hcode".
+    { split; auto; solve_addr. }
+    iEval (cbn) in "Hct1".
+    (* geta ctp ct1; *)
+    iInstr "Hcode".
+    (* lt ctp ctp MemNum; (* ctp := if (ctp < MemNum) then 1 else 0 *) *)
+    iInstr "Hcode".
+
+    destruct ( ((0 ^+ next_free_uk)%a <? 2000000)%Z ) eqn:Hnext_free_uk; iEval (cbn) in "Hctp".
+    - apply Z.ltb_lt in Hnext_free_uk.
+      assert ( (next_free_uk <? MemNum)%Z = true ) as Hnext_free_uk_true.
+      { Transparent MemNum.
+        rewrite /MemNum.
+        apply Z.ltb_lt.
+        admit.
+      }
+      rewrite Hnext_free_uk_true.
+      (* jnz (".initialise_next_free_available")%asm ctp; *)
+      iInstr "Hcode".
+      (* mov ca0 ASM_SOME; *)
+      iInstr "Hcode".
+      (* seal ca1 ct0 ct1; *)
+      iInstr "Hcode"; auto.
+      { pose proof KVS_OTYPE_size; solve_addr. }
+      (* lea ct1 1; *)
+      iInstr "Hcode".
+      { transitivity (Some (0 ^+ (next_free_uk + 1)%Z)%a); auto.
+        admit.
+      }
+      (* store cgp ct1; *)
+      iInstr_lookup "Hcode" as "Hi" "Hcode".
+      wp_instr.
+      iApply (rules_Store.wp_store_success_reg with "[$HPC $Hi $Hct1 $Hcgp $Ha_next_free_uk]")
+      ; try solve_pure; auto.
+      { solve_addr. }
+      iNext; iIntros "(HPC & Hi & Hct1 & Hcgp & Ha_next_free_uk)".
+      wp_pure.
+      iInstr_close "Hcode".
+      (* ret *)
+      iInstr "Hcode".
+      subst hcont; unfocus_block "Hcode" "Hcont" as "Hcode".
+
+      iApply "Hpost".
+      iFrame "HPC Hcgp Hcra Hca0 Hca1 Hct1 Hct0 Hctp Hcnull Hcode Ha_unsealing Ha_next_free_uk".
+      rewrite seqZ_cons.
+      { iDestruct "Hnext_free_alloc" as "[$ H]".
+        by replace ( (Z.pred (MemNum - next_free_uk)) ) with (MemNum - (next_free_uk + 1))%Z by lia.
+      }
+      Transparent MemNum.
+      rewrite /MemNum.
+      rewrite /MemNum in Hnext_free_uk_true.
+      apply Z.ltb_lt in Hnext_free_uk_true.
+      lia.
+
+    - apply Z.ltb_ge in Hnext_free_uk.
+      assert ( (next_free_uk <? MemNum)%Z = false ) as ->.
+      { Transparent MemNum.
+        rewrite /MemNum.
+        apply Z.ltb_ge.
+        admit.
+      }
+      (* jnz (".initialise_next_free_available")%asm ctp; *)
+      iInstr "Hcode".
+      (* mov ca0 ASM_NONE; *)
+      iInstr "Hcode".
+      (* ret; *)
+      iInstr "Hcode".
+      subst hcont; unfocus_block "Hcode" "Hcont" as "Hcode".
+
+      iApply "Hpost".
+      iFrame "HPC Hcgp Hcra Hca0 Hca1 Hct1 Hct0 Hctp Hcnull Hcode Ha_unsealing Ha_next_free_uk Hnext_free_alloc".
+  Admitted.
+
+  Lemma KVS_initialise_spec_in
+    (wret : Word)
+    (E : coPset)
+    :
+
+    ↑Nkvs ⊆ E ->
+
+    ( na_inv cerise_nais Nkvs kvs_inv ∗
+      na_own cerise_nais E ∗
+
+      (* initial register file *)
+      PC ↦ᵣ WCap RX Global KVS_pcc_b KVS_pcc_e kvs_initialise_pcc_addr ∗
+      cgp ↦ᵣ WCap RW Global KVS_cgp_b KVS_cgp_e KVS_cgp_b ∗
+      cra ↦ᵣ wret ∗
+      ca0 ↦ᵣ - ∗
+      ca1 ↦ᵣ - ∗
+      ct0 ↦ᵣ - ∗ (* scratch *)
+      ct1 ↦ᵣ - ∗ (* scratch *)
+      ctp ↦ᵣ - ∗ (* scratch *)
+      cnull ↦ᵣ - ∗
+
+      ▷ (na_own cerise_nais E ∗
+         PC ↦ᵣ updatePcPerm wret ∗
+         cgp ↦ᵣ - ∗
+         cra ↦ᵣ - ∗
+         ct0 ↦ᵣ - ∗ (* scratch *)
+         ct1 ↦ᵣ - ∗ (* scratch *)
+         ctp ↦ᵣ - ∗ (* scratch *)
+         cnull ↦ᵣ - ∗
+         (
+           ( ∃ next_free_uk,
+               ⌜ (next_free_uk <? MemNum)%Z ⌝ ∗
+               ca0 ↦ᵣ WInt ASM_SOME ∗
+               ca1 ↦ᵣ (kvs_user_seal_key Global next_free_uk) ∗
+               ◯(ALLOC)[next_free_uk] ∅
+           )
+           ∨
+             (
+               ca0 ↦ᵣ WInt ASM_NONE ∗
+               ca1 ↦ᵣ -
+             )
+         )
+
+         -∗ WP Seq (Instr Executable) {{ v, ⌜v = HaltedV⌝ → na_own cerise_nais ⊤ }}
+        )
+      ⊢ WP Seq (Instr Executable) {{ v, ⌜v = HaltedV⌝ → na_own cerise_nais ⊤ }})%I.
+  Proof.
+    iIntros (Hnkvs_E)
+      "(#Hkvs_inv & Hna & HPC & Hcgp & Hcra & Hca0 & Hca1 & Hct0 & Hct1 & Hctp & Hcnull & Hpost)".
+    iMod (na_inv_acc with "Hkvs_inv Hna")
+      as "( (%m & %s & %next_free_uk & >Himports & >Hcgp_e & >Hcode & HisKVS & Hfree_uk_alloc & #Hspred) & Hna & Hkvs_inv_close)"; eauto.
+    pose proof (Hcgp_continuous := KVS_size_data).
+    pose proof (HKVS_pcc_b' := KVS_size_imports).
+    pose proof (Hcode_continuous := KVS_size_code).
+    assert (SubBounds KVS_pcc_b KVS_pcc_e kvs_initialise_pcc_addr (kvs_initialise_pcc_addr ^+ length kvs_initialise_instrs)%a) as HSubBounds.
+    { rewrite /kvs_initialise_pcc_addr; cbn in *; solve_addr. }
+    codefrag_facts "Hcode"; rename H into Hpc_contiguous.
+    rewrite /kvs_imports /kvs.kvs_imports_pre.
+    assert ((KVS_pcc_b + 1)%a = Some (KVS_pcc_b ^+ 1)%a) by ( rewrite /length_kvs_imports in HKVS_pcc_b'; solve_addr+ HKVS_pcc_b').
+    assert ((KVS_pcc_b ^+ 1)%a <= KVS_pcc_b')%a  by ( rewrite /length_kvs_imports in HKVS_pcc_b'; solve_addr+ HKVS_pcc_b').
+    assert ((KVS_pcc_b ^+ 1 + 1)%a = Some (KVS_pcc_b')%a) by ( rewrite /length_kvs_imports in HKVS_pcc_b'; solve_addr+ HKVS_pcc_b').
+    iDestruct (region_pointsto_cons with "Himports") as "[Himports_sw Himports]"; eauto.
+    iDestruct (region_pointsto_single with "Himports") as "(% & Ha_unsealing & %Heq)"; eauto; simplify_eq.
+
+    rewrite /kvs_service_instrs.
+    focus_block_nochangePC 3 "Hcode" as a_initialise Ha_initialise "Hcode" "Hcont"; iHide "Hcont" as hcont.
+    assert (a_initialise = kvs_initialise_pcc_addr) as -> by (rewrite /kvs_initialise_pcc_addr ; cbn in * ; solve_addr+Hcode_continuous HKVS_pcc_b' Ha_initialise).
+    replace (KVS_pcc_b ^+ 1)%a with (KVS_pcc_b ^+ UNSEALING_USER_KEY_OFFSET)%a by (rewrite /UNSEALING_USER_KEY_OFFSET; solve_addr+).
+    iApply (KVS_initialise_spec_pre with "[- $HPC]"); last iFrame; eauto.
+    iNext; iIntros "(HPC & Hcgp & Hcra & Hca0 & Hca1 & Hctp & Hct0 & Hct1
+              & Hcnull & Hcode & Ha_unsealing & Hcgp_e & Hfree_uk_alloc)".
+    subst hcont; unfocus_block "Hcode" "Hcont" as "Hcode".
+
+    destruct ( (next_free_uk <? MemNum)%Z ) eqn:Hfree.
+    - iDestruct "Hfree_uk_alloc" as "[Hfree_uk_alloc Halloc]".
+      iMod ("Hkvs_inv_close" with "[$Hcode $Hcgp_e Himports_sw Ha_unsealing $HisKVS $Hfree_uk_alloc $Hspred $Hna]") as "Hna" ; auto.
+      { iNext.
+        iApply (region_pointsto_cons with "[Ha_unsealing Himports_sw]"); eauto; iFrame.
+        iApply (region_pointsto_cons with "[Ha_unsealing]"); eauto; [solve_addr+|]; iFrame.
+        rewrite /region_pointsto finz_seq_between_empty; auto; solve_addr+.
+      }
+      iApply "Hpost"; iFrame.
+      iLeft; iFrame.
+      iPureIntro; rewrite Hfree; auto.
+    - iMod ("Hkvs_inv_close" with "[$Hcode $Hcgp_e Himports_sw Ha_unsealing $HisKVS $Hfree_uk_alloc $Hspred $Hna]") as "Hna" ; auto.
+      { iNext.
+        iApply (region_pointsto_cons with "[Ha_unsealing Himports_sw]"); eauto; iFrame.
+        iApply (region_pointsto_cons with "[Ha_unsealing]"); eauto; [solve_addr+|]; iFrame.
+        rewrite /region_pointsto finz_seq_between_empty; auto; solve_addr+.
+      }
+      iApply "Hpost"; iFrame.
+      iRight; iFrame.
+  Qed.
+
+End KVS_spec_initialise.
