theories/case_studies/multiuser_kvs/kvs_spec_read_safe.v
@@ -32,7 +32,7 @@ Section KVS_spec_read_safe.
     ↑Nkvs_otype ⊆ E ->
 
     SubBounds pc_b pc_e pc_a (pc_a ^+ length kvs_read_instrs)%a ->
-    (cgp_b + length kvs_data)%a = Some cgp_e ->
+    (cgp_b + length_kvs_data)%a = Some cgp_e ->
 
     related_sts_priv_world Wca0 W ->
 
@@ -87,6 +87,7 @@ Section KVS_spec_read_safe.
     iIntros (HN HsubBounds Hcgp_contiguous Hrelated_Wca0_W)
       "(Hna & HPC & Hcgp & Hcra & Hca0 & #Hinterp_wca0 & Hca1 & Hct1 & Hct2 & Hctp & [%wcnull Hcnull] &
         Hcode & Ha_unsealing & HKVS & #Hspred & Hworld & Hpost)".
+    rewrite /length_kvs_data /= in Hcgp_contiguous.
     codefrag_facts "Hcode"; rename H into Hpc_contiguous ; clear H0.
 
     (* --------------------------------------------------- *)
@@ -307,7 +308,7 @@ Section KVS_spec_read_safe.
       "(#Hkvs_inv & Hna & HPC & Hcgp & Hcra & Hca0 & Hinterp_ca0
       & Hca1 & Hct1 & Hct2 & Hctp & Hcnull & Hworld & Hpost)".
     iMod (na_inv_acc with "Hkvs_inv Hna")
-      as "( (%m & %s & >Himports & >Hcode & HisKVS & #Hspred) & Hna & Hkvs_inv_close)"; eauto.
+      as "( (%m & %s & %next_free_uk & >Himports & >Hcgp_e & >Hcode & HisKVS & Hfree_uk_alloc & #Hspred) & Hna & Hkvs_inv_close)"; eauto.
     pose proof (Hcgp_continuous := KVS_size_data).
     pose proof (HKVS_pcc_b' := KVS_size_imports).
     pose proof (Hcode_continuous := KVS_size_code).
@@ -332,7 +333,7 @@ Section KVS_spec_read_safe.
     subst hcont; unfocus_block "Hcode" "Hcont" as "Hcode".
 
     iDestruct "Hres" as "[ (%w & Hca0 & Hca1 & Hinterp_w) | (Hca0 & Hca1) ]".
-    all: iMod ("Hkvs_inv_close" with "[$Hna $Hcode Himports_sw Ha_unsealing $HKVS $Hspred]") as "Hna"
+    all: iMod ("Hkvs_inv_close" with "[$Hcode $Hcgp_e Himports_sw Ha_unsealing $HKVS $Hfree_uk_alloc $Hspred $Hna]") as "Hna"
     ; last ( iApply "Hpost"; iFrame); try (iLeft; iFrame).
     all: iNext.
     all: iApply (region_pointsto_cons with "[Ha_unsealing Himports_sw]"); eauto; iFrame.
